

Tutorial-4.

$$1) \quad f_x(n) = c n e^{-n/2}, \quad n \geq 0 \\ = 0, \quad n < 0$$

(i) $\therefore f_x(n)$ is pdf, then.

$$\int_{-\infty}^{\infty} f_x(n) dn = 1$$

$$\Rightarrow \int_0^{\infty} c \cdot n \cdot e^{-n/2} dn = 1$$

$$\Rightarrow c \int_0^{\infty} n e^{-n/2} dn = 1$$

$$\Rightarrow c \cdot \left[\left[n \int e^{-n/2} dn \right]_0^{\infty} - \int_0^{\infty} \left[\frac{d}{dn} \cdot \int e^{-n/2} dn \right] dn \right] = 1$$

$$\Rightarrow c \left[\left[-n \cdot 2 \cdot e^{-n/2} \right]_0^{\infty} + \int_0^{\infty} 2 e^{-n/2} dn \right] = 1$$

$$\Rightarrow c \left[0 + 2 \int_0^{\infty} e^{-n/2} dn \right] = 1$$

$$\Rightarrow 2c \cdot 2 \left[-e^{-n/2} \right]_0^{\infty} = 1$$

$$\Rightarrow 2c \cdot 2 \cdot [0 + 1] = 1$$

$$\Rightarrow c = \frac{1}{4}$$

$$(ii) \quad F_x(n) = \int_{-\infty}^n f_x(t) dt$$

$$\therefore F_x(n) = 0, \quad n < 0$$

$$= \int_0^n \frac{1}{4} \cdot t \cdot e^{-t/2} dt, \quad n \geq 0$$

$$= \frac{1}{4} \int_0^{\infty} t \cdot e^{-\frac{t}{2}} dt$$

$$= \frac{1}{4} \cdot \int_0^{\infty} t e^{-\frac{t}{2}} dt$$

$$= \frac{1}{4} \left[\left[t \cdot \int e^{-\frac{t}{2}} dt \right]_0^{\infty} - \int_0^{\infty} \left[\frac{d}{dt} (t) \cdot \int e^{-\frac{t}{2}} dt \right] dt \right] =$$

$$= \frac{1}{4} \left[\left[2t \cdot \left[-e^{-\frac{t}{2}} \right] \right]_0^{\infty} + 2 \int_0^{\infty} e^{-\frac{t}{2}} dt \right]$$

$$= \frac{1}{4} \left[-2\infty e^{-\frac{\infty}{2}} + -4 \cdot \left[e^{-\frac{\infty}{2}} - 1 \right] \right]$$

$$= \frac{1}{2} \left[-\infty e^{-\frac{\infty}{2}} - 2e^{-\frac{\infty}{2}} + 2 \right]$$

$$\therefore F_X(m) = 0, m < 0$$

$$= \frac{1}{2} \left[-\infty e^{-\frac{\infty}{2}} - 2e^{-\frac{\infty}{2}} + 2 \right], m \geq 0$$

$$(iii) E(X) = \int_{-\infty}^{\infty} m \cdot f_X(m) dm$$

$$= \int_0^{\infty} m \cdot f_X(m) dm$$

$$= \frac{1}{4} \int_0^{\infty} m \cdot m \cdot e^{-\frac{m}{2}} dm \quad \left[\begin{array}{l} \because f_X(m) = \frac{1}{4} m e^{-\frac{m}{2}} \quad m \geq 0 \\ = 0 \quad m < 0 \end{array} \right]$$

$$= \frac{1}{4} \int_0^{\infty} m^2 e^{-\frac{m}{2}} dm$$

$$= \frac{1}{4} \left[\left[m^2 \int e^{-\frac{m}{2}} dm \right]_0^{\infty} - \int_0^{\infty} \left[\frac{d}{dm} (m^2) \int e^{-\frac{m}{2}} dm \right] dm \right]$$

$$= \frac{1}{4} \left[\left[n^2 \cdot 2 \left[-e^{-\frac{n}{2}} \right] \right]_0^\infty + 4 \int_0^\infty n \cdot e^{-\frac{n}{2}} dn \right]$$

$$= \frac{1}{4} \times 4 \int_0^\infty n \cdot e^{-\frac{n}{2}} dn$$

$$= \left[-2n \cdot e^{-\frac{n}{2}} \right]_0^\infty + 2 \int_0^\infty e^{-\frac{n}{2}} dn$$

$$= 2 \times \left[-2 \cdot e^{-\frac{n}{2}} \right]_0^\infty$$

$$= 4.$$

$$\text{Therefore } E(x^2) = \frac{1}{4} \int_0^\infty n^2 \cdot n \cdot e^{-\frac{n}{2}} dn$$

$$= \frac{1}{4} \int_0^\infty n^3 e^{-\frac{n}{2}} dn$$

$$= \frac{1}{4} \left[\left[-2n^3 e^{-\frac{n}{2}} \right]_0^\infty - \int_0^\infty [3n^2 \cdot \int e^{-\frac{n}{2}} dn] dn \right]$$

$$= \frac{1}{4} \left[3 \times 2 \int_0^\infty n^2 e^{-\frac{n}{2}} dn \right]$$

$$= \frac{1}{4} \times 6 \cdot 4 \times E(x)$$

$$= 6 \times 4$$

$$= 24$$

$$\therefore V(x) = E(x^2) - \{E(x)\}^2 = 24 - (4)^2$$

$$= 24 - 16$$

$$= 8$$

$$S.D.(X) = \sqrt{V(X)} = \sqrt{8} = 2\sqrt{2}$$

iv) For continuous random variable, if μ is median, then,

$$F_X(\mu) = \frac{1}{2}$$

$$\Rightarrow \frac{1}{2} [-\mu e^{-\frac{\mu}{2}} - 2e^{-\frac{\mu}{2}} + 2] = \frac{1}{2}$$

$$\Rightarrow -\mu e^{-\frac{\mu}{2}} - 2e^{-\frac{\mu}{2}} + 2 = 1$$

$$\Rightarrow (\mu + 2) e^{-\frac{\mu}{2}} = 1$$

$$\Rightarrow (\mu + 2) = e^{\frac{\mu}{2}}$$

$$\Rightarrow (\mu + 2) - e^{\frac{\mu}{2}} = 0$$

Solve this eqⁿ numerically. [use Newton Raphson with interval $[-6, 6]$]

2) X : The distance between the dart's impact point and the center of the target.

$$P(X \leq x) = c\pi x^2, \quad 0 \leq x \leq 25$$

$$= 1, \quad x > 25$$

(i) C D F of X is

$$F_X(x) = \begin{cases} 0 & x < 0 \\ c\pi x^2 & 0 \leq x \leq 25 \\ 1 & x > 25 \end{cases}$$

$$\therefore f_X(x) = \frac{d}{dx} F_X(x) = \frac{d}{dx} (c\pi x^2) = 2c\pi x \quad \text{when } 0 \leq x \leq 25$$

$$\therefore f_X(x) = \begin{cases} 2c\pi x & 0 \leq x \leq 25 \\ 0 & \text{otherwise} \end{cases}$$

$$\therefore \int_{-\infty}^{\infty} f_x(m) dm = 1$$

$$\Rightarrow \int_0^{25} 2cm dm = 1$$

$$\Rightarrow 2c\pi \left[\frac{m^2}{2} \right]_0^{25} = 1$$

$$\Rightarrow c = \frac{1}{(25)^2 \pi}$$

$$= \frac{1}{625 \pi}$$

(ii) P.D.F of x is $f_x(m) = \frac{2}{625} m$
 $= 0$

$$0 \leq m \leq 25$$

otherwise

(iii) $E(x) = \int_{-\infty}^{\infty} x f_x(m) dm$
 $= \int_0^{25} m \cdot \frac{2}{625} m dm$
 $= \frac{2}{625} \left[\frac{m^3}{3} \right]_0^{25}$
 $= \frac{25 \times 2 \times 25}{3}$
 $= \frac{50}{3}$

$$\begin{aligned}
 \text{(iv)} \quad P(X \leq 10 | X \geq 5) &= \frac{P(5 \leq X \leq 10)}{P(X \geq 5)} \\
 &= \frac{P(5 \leq X \leq 10)}{1 - P(X < 5)} \\
 &= \frac{\int_5^{10} f_x(m) dm}{1 - \int_0^5 f_x(m) dm} \\
 &= \frac{\int_5^{10} \frac{2}{625} x dm}{1 - \int_0^5 \frac{2}{625} x dm} \\
 &= \frac{\frac{2}{625} \left[\frac{x^2}{2} \right]_5^{10}}{1 - \frac{2}{625} \left[\frac{x^2}{2} \right]_0^5} \\
 &= \frac{\frac{21}{625} (10^2 - 5^2)}{1 - \frac{1}{625} \times 25} \\
 &= \frac{10^2 - 5^2}{8625 - 25} \\
 &= \frac{5 \times 15}{600} \\
 &= \frac{1}{8}
 \end{aligned}$$

$$\text{(v)} \quad 10 \times \int_0^r x \cdot \frac{2}{625} x dm + 1 \times \int_r^{2r} x \cdot \frac{2}{625} x dm + 0 \times \int_{2r}^{2r} x \cdot \frac{2}{625} x dm = 1 + 0.25$$

$$\Rightarrow \frac{2}{625} \times \frac{1}{3} [10r^3 + 8r^3 - r^3] = 1.25$$

$$\Rightarrow r^3 = \frac{3 \times 625 \times 1.25}{2 \times 17}$$

3)

$$f_x(n) = \frac{n(6+n)}{3(3+n)^2}, \quad 0 < n \leq 3$$

$$= \frac{9(3+2n)}{n^2(3+n)^2}, \quad n > 3$$

$$\begin{aligned} \int_{-\infty}^{\infty} f_x(n) dn &= \int_0^3 \frac{n(6+n)}{3(3+n)^2} dn + \int_3^{\infty} \frac{9(3+2n)}{n^2(3+n)^2} dn \\ &= \int_0^3 \frac{n^2+6n}{3(3+n)^2} dn + \int_3^{\infty} \frac{9(3+2n)}{(3n+n^2)^2} dn \\ &= \int_0^3 \frac{n^2+6n+9-9}{3(3+n)^2} dn + \int_3^{\infty} \frac{9(3+2n)}{(3n+n^2)^2} dn \\ &= \int_0^3 \frac{1}{3} dn - \int_0^3 \frac{1}{(3+n)^2} dn + \int_3^{\infty} \frac{9 d(3n+n^2)}{(3n+n^2)^2} \\ &= \left[\frac{n}{3} \right]_0^3 + 3 \left[\frac{1}{(3+n)} \right]_0^3 - \left[\frac{9}{(3n+n^2)} \right]_3^{\infty} \\ &= 1 + \frac{1}{2} - 1 + \frac{9}{18} \\ &= 1 \end{aligned}$$

$\therefore f_x(n)$ is a pdf.

4)

$$f_x(n) = \theta^2 n e^{-\theta n}, \quad n > 0$$

$$= 0, \quad n \leq 0$$

$$\begin{aligned} \int_{-\infty}^{\infty} f_x(n) dn &= \int_0^{\infty} \theta^2 n e^{-\theta n} dn \\ &= \theta^2 \int_0^{\infty} n e^{-\theta n} dn \\ &= \theta^2 \left[\left[-\frac{n e^{-\theta n}}{\theta} \right]_0^{\infty} + \frac{1}{\theta} \int_0^{\infty} e^{-\theta n} dn \right] \\ &= \theta^2 \times \frac{1}{\theta} \cdot \left[-e^{-\theta n} \right]_0^{\infty} \\ &= \frac{1}{\theta^2} \times \theta^2 \\ &= 1. \end{aligned}$$

$\therefore f_x(n)$ is a pdf.

$$\begin{aligned} F_x(n) &= \int_{-\infty}^n f_x(t) dt \\ &= \int_0^n \theta^2 t e^{-\theta t} dt \\ &= \theta^2 \int_0^n t e^{-\theta t} dt \\ &= \theta^2 \left\{ \left[\frac{t e^{-\theta t}}{-\theta} \right]_0^n + \frac{1}{\theta} \int_0^n e^{-\theta t} dt \right\} \\ &= \theta^2 \left[-\frac{n e^{-\theta n}}{\theta} - \frac{1}{\theta^2} [e^{-\theta n} - 1] \right] \\ &= 1 - e^{-\theta n} - n \theta e^{-\theta n} \\ &= 1 - e^{-\theta n} (1 + n \theta) \end{aligned}$$

$$\begin{aligned}
 P(X \geq 1) &= 1 - P(X < 1) \\
 &= 1 - [1 - e^{-\theta(\theta+1)}] \\
 &= e^{-\theta(\theta+1)}
 \end{aligned}$$

$$\begin{aligned}
 5) \quad i) \quad F(m) &= 0 \quad m \leq 0 \\
 &= \frac{m}{2} \quad 0 \leq m < 1 \\
 &= \frac{1}{2} \quad 1 \leq m < 2 \\
 &= \frac{m}{4} \quad 2 \leq m < 4 \\
 &= 1 \quad m \geq 4
 \end{aligned}$$

$F(m)$ is right continuous and non decreasing
 $F(-\infty) = 0$
 and $F(\infty) = 1$

$\therefore F(m)$ is C.D.F.

$$\frac{d}{dm}(F(m)) = \frac{d}{dm}\left(\frac{m}{2}\right) = \frac{1}{2} \quad \text{when } 0 \leq m < 1$$

$$\frac{d}{dm}(F(m)) = \frac{d}{dm}\left(\frac{m}{4}\right) = \frac{1}{4} \quad 2 \leq m < 4$$

$$\begin{aligned}
 \therefore f_x(m) &= \frac{1}{2} \quad 0 \leq m < 1 \\
 &= \frac{1}{4} \quad 2 \leq m < 4 \\
 &= 0 \quad \text{otherwise}
 \end{aligned}$$

$$\begin{aligned}
 \text{(ii)} \quad F(x) &= 0, \quad x < -\theta \\
 &= \frac{1}{2} \left(\frac{x}{\theta} + 1 \right), \quad |x| \leq \theta \\
 &= 1, \quad x > \theta
 \end{aligned}$$

$F(x)$ is right continuous and non decreasing.

$$\text{Also, } F(-\infty) = 0$$

$$F(\infty) = 1$$

$\therefore F(x)$ is a CDF

$$\frac{d}{dx} (F(x)) = \frac{d}{dx} \left(\frac{1}{2} \left(\frac{x}{\theta} + 1 \right) \right) = \frac{1}{2\theta} \quad \text{when } |x| \leq \theta$$

$$\begin{aligned}
 \therefore f_x(x) &= \frac{1}{2\theta} \quad |x| \leq \theta \\
 &= 0 \quad \text{otherwise}
 \end{aligned}$$

$$\text{(iii)} \quad F(x) = 0 \quad x < 1$$

$$= \frac{(x-1)^2}{8} \quad 1 \leq x < 3$$

$$= 1 \quad x \geq 3$$

$F(x)$ is right continuous everywhere except at $x=3$ and $F(x)$ is non decreasing. Also $F(-\infty) = 0$ and $F(\infty) = 1$.
 $\therefore F(x)$ is a CDF. At $x=3$, $F(3-0) - F(3) = P(X=3)$
 $\Rightarrow P(X=3) = \frac{1}{2}$

$$\frac{d}{dx} (F(x)) = \frac{2(x-1)}{8} = \frac{(x-1)}{4} \quad 1 \leq x < 3$$

$$\begin{aligned}
 \therefore f_x(x) &= \frac{x-1}{4} \quad 1 \leq x < 3 \\
 &= \frac{1}{2} \quad x = 3 \\
 &= 0 \quad \text{elsewhere}
 \end{aligned}$$

6)

$$f(n) = \frac{\Gamma(m)}{\Gamma(1/2) \Gamma(m-1/2) (1+n^2)^m}, \quad -\infty < n < \infty, \quad m \geq 1.$$

$$E(x^{2r}) = \int_{-\infty}^{\infty} x^{2r} \cdot f(n) \, dn$$

$$= \int_{-\infty}^{\infty} n^{2r} \cdot \frac{\Gamma(m)}{\Gamma(1/2) \Gamma(m-1/2) (1+n^2)^m} \, dn$$

$$= \frac{\Gamma(m)}{\Gamma(1/2) \Gamma(m-1/2)} \int_{-\infty}^{\infty} \frac{n^{2r}}{(1+n^2)^m} \, dn$$

$$= \frac{\Gamma(m)}{\Gamma(1/2) \Gamma(m-1/2)} \cdot 2 \int_0^{\infty} \frac{n^{2r}}{(1+n^2)^m} \, dn$$

$$= \frac{\Gamma(m)}{\Gamma(1/2) \Gamma(m-1/2)} \cdot 2 \int_0^{\infty} \frac{n^{2r-1} \, d(n^2)}{(1+n^2)^m}$$

$$= \frac{\Gamma(m)}{\Gamma(1/2) \Gamma(m-1/2)} \int_0^{\infty} \frac{(n^2)^{(r+1/2)-1}}{(1+n^2)^m} \, d(n^2)$$

$$= \frac{\Gamma(m)}{\Gamma(1/2) \Gamma(m-1/2)} \beta\left(r+\frac{1}{2}, m-r-\frac{1}{2}\right) \left[\because \beta(m, n) = \int_0^{\infty} \frac{x^{m-1}}{(1+x)^{m+n}} \, dx \right]$$

7) Let X has a symmetric distribution about a .

$$\therefore P(X \geq a+m) = P(X \leq a-n)$$

$$\Rightarrow 1 - F_X(a+m) = F_X(a-n)$$

$$\Rightarrow -\frac{d}{dn} F_X(a+m) = \frac{d}{dn} F_X(a-n)$$

$$\Rightarrow f_X(a+m) = f_X(a-n)$$

$$\text{Now } E[X-a] = \int_{-\infty}^{\infty} (m-a) f_X(m) dm$$

$$= \int_{-\infty}^a (m-a) f_X(m) dm + \int_a^{\infty} (m-a) f_X(m) dm$$

$$= I_1 + I_2$$

Now, let

$$\text{Now, } I_1 = \int_{-\infty}^a (m-a) f_X(m) dm$$

$$\text{Let } m-a = z$$

$$\Rightarrow dm = dz$$

$$\therefore I_1 = \int_{-\infty}^0 z \cdot f_X(z+a) dz$$

$$I_2 = \int_a^{\infty} (m-a) f_X(m) dm$$

$$\text{Let, } m-a = -z$$

$$dm = -dz$$

$$\therefore I_2 = \int_0^{\infty} z \cdot f_X(a-z) dz$$

$$= -\int_{-\infty}^0 z \cdot f_X(m-z) dz = -\int_{-\infty}^0 z \cdot f_X(a+z) dz = -I_1$$

$$\therefore E(X-c) = T_1 - T_1 \\ = 0$$

$$\Rightarrow E(X) - c = 0$$

$$\Rightarrow E(X) = c$$

$$8) (i) \int_0^{\infty} [1 - F(m)] dm - \int_{-\infty}^0 F(m) dm$$

$$= \left[[1 - F(m)] \cdot \int 1 \cdot dm \right]_0^{\infty} - \int_0^{\infty} \left[\frac{d}{dm} [1 - F(m)] \cdot \int 1 \cdot dm \right] dm \\ = \left[F(m) \cdot \int 1 \cdot dm \right]_{-\infty}^0 + \int_{-\infty}^0 \left[\frac{d}{dm} (F(m)) \cdot \int 1 \cdot dm \right] dm$$

$$= \left[m \cdot (1 - F(m)) \right]_0^{\infty} + \int_0^{\infty} m \cdot f_x(m) dm - \left[m F(m) \right]_{-\infty}^0 + \int_{-\infty}^0 m f_x(m) dm$$

$$= \left[m(1 - F(m)) \right]_0^{\infty} - \left[m F(-m) \right]_{-\infty}^0 + \int_{-\infty}^0 m \cdot f_x(m) dm$$

$$= \left[m(1 - F(m) - F(-m)) \right]_0^{\infty} + E(m)$$

Given that as $m \rightarrow \infty$ $m(1 - F(m) - F(-m)) \rightarrow 0$

$$\Rightarrow \int_0^{\infty} (1 - F(m)) dm - \int_{-\infty}^0 F(m) dm = E(X)$$

(ii) When X_m is non negative,

then, $F(m) = 0$ as $m < 0$

$$\text{Then } \int_{-\infty}^0 F(m) dm = 0$$

$$\therefore E(x) = \int_0^{\infty} (1 - F(m)) \, dm$$

$$g) \quad F(m) = 1 - 0.8 e^{-m}, \quad m \geq 0 \\ = 0, \quad m < 0$$

$$f_x(m) = \frac{d}{dm} (F(m)) = 0.8 \cdot e^{-m}$$

$$\therefore f_x(m) = 0, \quad m < 0 \\ = 1 - 0.8, \quad m = 0 \\ = 0.2, \quad m = 0 \\ = 0.8 \cdot e^{-m}, \quad m > 0$$

$$E(x) = \int_{-\infty}^{\infty} m \cdot f_x(m) \, dm + 0 \times P(x=0) + \int_0^{\infty} m \cdot f_x(m) \, dm$$

$$= \int_0^{\infty} 0 + 0 \times 0.2 + \int_0^{\infty} m \cdot 0.8 \cdot e^{-m} \, dm$$

$$= (0.8) \int_0^{\infty} m e^{-m} \, dm$$

$$= 0.8 \left[\left[-m e^{-m} \right]_0^{\infty} + \int_0^{\infty} e^{-m} \, dm \right]$$

$$= 0.8 \times \left[-e^{-m} \right]_0^{\infty}$$

$$= 0.8$$

$$10) \quad f(x) = \frac{1}{2} \quad -1 \leq x \leq 1$$

$$= 0 \quad \text{otherwise}$$

$$Y = \max(X, 0)$$

$$\therefore Y = 0 \quad x \leq 0$$

$$= x \quad \text{when } x \geq 0$$

Now, $P(Y \leq y) = \int_{-\infty}^y f(x) dx$ not

$$= \int_{-\infty}^y \frac{1}{2} dx$$

$$= \frac{y+1}{2}$$

$$F(y) = P(Y \leq y) = \int_{-\infty}^y f(x) dx$$

$$= \int_{-\infty}^y \frac{1}{2} dx$$

$$= \frac{1}{2} (y+1) \quad -1 \leq y \leq 1$$

$$F(y) = \frac{1}{2} (y+1) \quad -1 \leq y \leq 1$$

$$= 0 \quad \text{elsewhere}$$

$$11) f_x(n) = \frac{1}{2a} e^{-\frac{|n-\mu|}{a}}, \quad -\alpha < n < \alpha, \quad a > 0$$

$-\alpha < \mu < \alpha$

$$\begin{aligned} \int_{-\alpha}^{\alpha} f_x(n) dn &= \int_{-\alpha}^{\alpha} \frac{1}{2a} e^{-\frac{|n-\mu|}{a}} dn \\ &= \int_{-\alpha}^{\mu} \frac{1}{2a} e^{-\frac{-(n-\mu)}{a}} dn + \int_{\mu}^{\alpha} \frac{1}{2a} e^{-\frac{(n-\mu)}{a}} dn \\ &= \frac{1}{2a} \int_{-\alpha}^{\mu} e^{\frac{(n-\mu)}{a}} dn + \int_{\mu}^{\alpha} \frac{1}{2a} e^{-\frac{(n-\mu)}{a}} dn \\ &= \frac{1}{2a} \cdot a \left[e^{\frac{n-\mu}{a}} \right]_{-\alpha}^{\mu} + -\frac{1}{2a} \cdot a \left[e^{-\frac{(n-\mu)}{a}} \right]_{\mu}^{\alpha} \\ &= \frac{1}{2a} \cdot a + \frac{1}{2a} \cdot a = 1 \end{aligned}$$

$\therefore f_x(n)$ is pdf.

$$\begin{aligned} M_x(t) &= E(e^{tx}) = \int_{-\alpha}^{\alpha} e^{tn} f_x(n) dn \\ &= \frac{1}{2a} \int_{-\alpha}^{\mu} e^{tn} e^{\frac{(n-\mu)}{a}} dn + \frac{1}{2a} \int_{\mu}^{\alpha} e^{tn} e^{-\frac{(n-\mu)}{a}} dn \\ &= \frac{1}{2a} \left[\int_{-\alpha}^{\mu} e^{(t+\frac{1}{a})n - \frac{\mu}{a}} dn + \int_{\mu}^{\alpha} e^{(t-\frac{1}{a})n + \frac{\mu}{a}} dn \right] \\ &= \frac{1}{2a} \left\{ \left[\frac{a}{(at+1)} e^{(t+\frac{1}{a})n - \frac{\mu}{a}} \right]_{-\alpha}^{\mu} + \left[\frac{a}{(at-1)} e^{(t-\frac{1}{a})n + \frac{\mu}{a}} \right]_{\mu}^{\alpha} \right\} \\ &= \frac{1}{2a} \left[\frac{a}{(at+1)} e^{t\mu} + \frac{a}{(at-1)} e^{\frac{\mu}{a}} \right] \\ &= \frac{1}{2} e^{t\mu} \left[\frac{1}{at+1} + \frac{1}{at-1} \right] \end{aligned}$$

$$= \frac{1}{2} \cdot e^{at} \cdot \frac{2at}{(a^2 t^2 - 1)}$$

$$= \frac{at e^{at}}{(a^2 t^2 - 1)}$$

$$12) f_x(n) = \frac{1}{2} \left[1 - \frac{|n-3|}{2} \right], \quad 1 \leq n \leq 5$$

$$\int_{-\infty}^{\infty} f_x(n) dn = \int_1^5 \frac{1}{2} \left(1 - \frac{|n-3|}{2} \right) dn$$

$$= \frac{1}{2} \int_1^3 \left[1 + \frac{(n-3)}{2} \right] dn + \frac{1}{2} \int_3^5 \left(1 - \frac{(n-3)}{2} \right) dn$$

$$= \frac{1}{2} \left[\int_1^3 \left(\frac{n}{2} - \frac{1}{2} \right) dn + \int_3^5 \left(\frac{5}{2} - \frac{n}{2} \right) dn \right]$$

$$= \frac{1}{2} \left\{ \left[\frac{n^2}{4} - \frac{n}{2} \right]_1^3 + \left[\frac{5n}{2} - \frac{n^2}{4} \right]_3^5 \right\}$$

$$= \frac{1}{2} \left[\frac{9}{4} - \frac{3}{2} - \frac{1}{4} + \frac{1}{2} + \frac{25}{2} - \frac{25}{4} - \frac{15}{2} + \frac{9}{4} \right]$$

$$= \frac{1}{2} \times 2$$

$$= 1$$

$\therefore f_x(n)$ is a ~~pdf~~ PDF

$$E(x) = \int_{-\infty}^{\infty} n \cdot f_x(n) dn$$

$$= \frac{1}{2} \int_1^5 n \cdot \left[1 - \frac{|n-3|}{2} \right] dn$$

$$\begin{aligned}
&= \frac{1}{2} \left\{ \int_1^3 n \left(1 + \frac{n-3}{2}\right) dn + \int_3^5 n \left(1 - \frac{n-3}{2}\right) dn \right\} \\
&= \frac{1}{2} \left\{ \int_1^3 \left(\frac{n^2}{2} - \frac{n}{2}\right) dn + \int_3^5 \left(\frac{5n}{2} - \frac{n^2}{2}\right) dn \right\} \\
&= \frac{1}{2} \left\{ \left[\frac{n^3}{6} - \frac{n^2}{4} \right]_1^3 + \left[\frac{5n^2}{4} - \frac{n^3}{6} \right]_3^5 \right\} \\
&= \frac{1}{2} \left[\frac{27}{6} - \frac{9}{4} - \frac{1}{6} + \frac{1}{4} + \frac{125}{4} - \frac{125}{6} - \frac{45}{4} + \frac{27}{6} \right] \\
&= \frac{1}{2} \times 6 \\
&= 3
\end{aligned}$$

For median,

$$\begin{aligned}
&\int_1^n \frac{1}{2} \left[1 - \frac{|t-3|}{2} \right] dt = \frac{1}{2} \\
\Rightarrow &\int_1^3 \frac{1}{2} \left[1 + \frac{(t-3)}{2} \right] dt + \int_3^n \frac{1}{2} \left[1 - \frac{(t-3)}{2} \right] dt = \frac{1}{2} \\
\Rightarrow &\int_1^3 \frac{1}{2} \left(\frac{t}{2} - \frac{5}{2} \right) dt + \int_3^n \left(\frac{5}{2} - \frac{t}{2} \right) dt = 1 \\
\Rightarrow &\left[\frac{t^2}{4} - \frac{5t}{2} \right]_1^3 + \left[\frac{5t}{2} - \frac{t^2}{4} \right]_3^n = 1 \\
\Rightarrow &\left[\frac{9}{4} - \frac{15}{2} - \frac{1}{4} + \frac{5}{2} \right] + \left[\frac{5n}{2} - \frac{n^2}{4} - \frac{15}{2} + \frac{9}{4} \right] = 1 \\
\Rightarrow &1 + \left[\frac{10n - n^2 - 21}{4} \right] = 1 \\
\Rightarrow &n^2 - 10n + 21 = 0 \\
\Rightarrow &(n-3)(n-7) = 0 \\
\Rightarrow &n=3. \therefore \text{Median is } n=3
\end{aligned}$$

$$\begin{aligned}
 E(x^2) &= \int_1^5 \frac{x^2}{2} \left[1 - \frac{|n-3|}{2} \right] dx \\
 &= \frac{1}{2} \int_1^3 x^2 \left(1 + \frac{n-3}{2} \right) dx + \frac{1}{2} \int_3^5 x^2 \left(1 - \frac{n-3}{2} \right) dx \\
 &= \frac{1}{2} \int_1^3 \left(\frac{x^3}{2} - \frac{x^2}{2} \right) dx + \frac{1}{2} \int_3^5 \left[\frac{5x^2}{2} - \frac{x^3}{2} \right] dx \\
 &= \frac{1}{2} \left\{ \left[\frac{x^4}{8} - \frac{x^3}{6} \right]_1^3 + \left[\frac{5x^3}{6} - \frac{x^4}{8} \right]_3^5 \right\} \\
 &= \frac{1}{2} \left[\frac{81}{8} - \frac{27}{6} - \frac{1}{8} + \frac{1}{6} + \frac{625}{6} - \frac{625}{8} - \frac{135}{8} + \frac{81}{8} \right] \\
 &= \frac{599}{48}
 \end{aligned}$$

$$\begin{aligned}
 V(x) &= \frac{599}{48} - 9[E(x)]^2 = \frac{599}{48} - 9 \\
 &= \frac{167}{48}
 \end{aligned}$$

p-th quantile

$$F_x(x_p) = p$$

$$\Rightarrow \int_1^{x_p} \frac{1}{2} \left[1 - \frac{|n-3|}{2} \right] dx = p$$

$$\Rightarrow \frac{1}{2} \int_1^3 \left(1 + \frac{n-3}{2} \right) dx + \frac{1}{2} \int_3^{x_p} \left(1 - \frac{n-3}{2} \right) dx = p$$

$$\Rightarrow \frac{1}{2} \left[\int_1^3 \left(\frac{n}{2} - \frac{1}{2} \right) dx + \int_3^{x_p} \left(\frac{5}{2} - \frac{n}{2} \right) dx \right] = p$$

$$\Rightarrow \frac{1}{2} \times \left[\frac{\frac{n^2}{4} - \frac{n}{2}}{1} \right]_1^3 + \frac{1}{2} \cdot \left[\frac{5n}{2} - \frac{n^2}{4} \right]_3^{x_p} = p$$

$$\Rightarrow \frac{1}{2} \left[\frac{9}{4} - \frac{3}{2} - \frac{1}{4} + \frac{1}{2} \right] + \frac{1}{2} \left[\frac{5m_p}{2} - \frac{m_p^2}{4} - \frac{15}{2} + \frac{9}{4} \right] = p$$

$$\Rightarrow \frac{1}{2} + \frac{1}{2} \left[\frac{10m_p - m_p^2 - 21}{4} \right] = p$$

$$\Rightarrow 4 + 10m_p - m_p^2 - 21 = 8p$$

$$\Rightarrow m_p^2 - 10m_p + 17p - 8p = 0$$

Solving this equation for given p gives the p th quantile.

13) $f_x(m) = \frac{K}{\beta} \left[1 - \frac{(m-\alpha)^2}{\beta^2} \right] \quad (\alpha-\beta) < m < (\alpha+\beta)$
 where $-\alpha < \alpha < \alpha$
 $\beta > 0$

$$\int_{-\alpha}^{\alpha} f_x(m) dm = \int_{-\alpha}^{\alpha} \frac{K}{\beta} \left[1 - \frac{(m-\alpha)^2}{\beta^2} \right] dm = 1$$

$$\Rightarrow \frac{K}{\beta} \int_{\alpha-\beta}^{\alpha+\beta} \left[1 - \frac{(m-\alpha)^2}{\beta^2} \right] dm = 1$$

$$\Rightarrow \frac{K}{\beta} \left[m - \frac{(m-\alpha)^3}{3\beta^2} \right]_{(\alpha-\beta)}^{(\alpha+\beta)} = 1$$

$$\Rightarrow \frac{K}{\beta} \left[(\alpha+\beta) - \frac{\beta^3}{3\beta^2} - (\alpha-\beta) + \frac{\beta^3}{3\beta^2} \right] = 1$$

$$\Rightarrow \frac{K}{\beta} \left[2\beta - \frac{\beta}{3} - \frac{\beta}{3} \right] = 1$$

$$\Rightarrow K \left[\frac{4}{3} \right] = 1$$

$$\Rightarrow K = \frac{3}{4}$$

$$E(x) = \int_{-\infty}^{\infty} x \cdot f_x(x) dx$$

$$= \int_{\alpha-\beta}^{\alpha+\beta} x \cdot \frac{3}{4\beta} \left[1 - \frac{(x-\alpha)^2}{\beta^2} \right] dx$$

$$= \frac{3}{4\beta} \int_{\alpha-\beta}^{\alpha+\beta} x \left[1 - \frac{(x-\alpha)^2}{\beta^2} \right] dx$$

$$= \frac{3}{4\beta} \int_{\alpha-\beta}^{\alpha+\beta} \left[x - \frac{x^3 - 2\alpha x^2 + \alpha^2 x}{\beta^2} \right] dx$$

$$= \frac{3}{4\beta} \left[\frac{x^2}{2} - \frac{x^3 - 2\alpha x^2 + \alpha^2 x}{3\beta^2} \right]_{\alpha-\beta}^{\alpha+\beta}$$

$$= \frac{3}{4\beta} \int_{\alpha-\beta}^{\alpha+\beta} \left[x - \frac{x^3 - 2\alpha x^2 + \alpha^2 x}{\beta^2} \right] dx$$

$$= \frac{3}{4\beta} \left[\frac{x^2}{2} - \frac{x^4}{4\beta^2} + \frac{2\alpha x^3}{3\beta^2} - \frac{\alpha^2 x^2}{2\beta^2} \right]_{(\alpha-\beta)}^{(\alpha+\beta)}$$

Median: $\int_{\alpha-\beta}^{\alpha} \frac{3}{4\beta} \left(1 - \frac{(t-\alpha)^2}{\beta^2} \right) dt = \frac{1}{2}$

$$\Rightarrow \frac{3}{4\beta} \left[t - \frac{(t-\alpha)^3}{3\beta^2} \right]_{(\alpha-\beta)}^{\alpha} = \frac{1}{2}$$

$$\Rightarrow \alpha - \frac{(n-\alpha)^3}{3\beta^2} - (\alpha-\beta) = \frac{\beta^3}{3\beta^2} = \frac{2\beta}{3}$$

$$\Rightarrow \alpha - \frac{(n-\alpha)^3}{3\beta^2} - \alpha + \beta - \frac{\beta}{3} = \frac{2\beta}{3}$$

$$\Rightarrow x - \frac{(x-\alpha)^2}{3\beta^2} = \alpha$$

$$\Rightarrow (x-\alpha) \left[1 - \frac{(x-\alpha)}{3\beta^2} \right] = 0$$

$\therefore x = \alpha$ is a median.

Variance

$$E(x^2) = \int_{-\alpha}^{\alpha} x^2 f_x(x) dx$$

$$= \int_{\alpha-\beta}^{\alpha+\beta} x^2 \cdot \frac{3}{4\beta} \left(1 - \frac{(x-\alpha)^2}{\beta^2} \right) dx$$

$$= \frac{3}{4\beta} \int_{\alpha-\beta}^{\alpha+\beta} \left(x^2 - \frac{x^4 - 2x^3\alpha + \alpha^2 x^2}{\beta^2} \right) dx$$

$$= \frac{3}{4\beta} \left[\frac{x^3}{3} - \frac{x^5}{5\beta^2} + \frac{2x^4\alpha}{4\beta^2} - \frac{\alpha^2 x^3}{3\beta^2} \right]_{(\alpha-\beta)}^{(\alpha+\beta)}$$

$$V(x) = E(x^2) - \{E(x)\}^2$$

p-th quantile

$$F(x_p) = p$$

$$\Rightarrow \frac{3}{4\beta} \int_{\alpha-\beta}^{x_p} \left(1 - \frac{(x-\alpha)^2}{\beta^2} \right) dx = p$$

$$\Rightarrow \int_{\alpha-\beta}^{x_p} \left(1 - \frac{(x-\alpha)^2}{\beta^2} \right) dx = \frac{3}{4\beta} p$$

$$\Rightarrow \left[\alpha - \frac{(\alpha - \alpha)^3}{3\beta^2} \right]_{(\alpha - \beta)}^{\alpha_p} = \frac{4\beta p}{3}$$

$$\Rightarrow \alpha_p - \frac{(\alpha_p - \alpha)^3}{3\beta^2} - (\alpha - \beta) = \frac{\beta^3}{3\beta^2} = \frac{4\beta p}{3}$$

$$\Rightarrow \frac{3\beta^2 \alpha_p - (\alpha_p - \alpha)^3}{3\beta^2} - \alpha + \beta - \frac{\beta}{3} = \frac{4\beta}{3} p$$

Solving this equation gives the p -th quantile